%!TEX root = ../main.tex
\documentclass[../main.tex]{subfiles}
\begin{document}

\subsection{Derivation of the optimal task choice} \label{app:derive_lmb_opt}
We start from the first order condition of the utility maximization:

\begin{equation}
	\frac{\partial u_{i, t}(b_i, \lambda_{i,t}, \phi, \theta, \tilde{w}_{i,t})}{\partial \lambda_{i,t}} = \tilde{w}_{i,t} + 2 \phi \theta \frac{(|b_i - \lambda_{i,t}|)^\phi}{b_i - \lambda_{i,t}} \overset{!}{=} 0 \tag{\ref{eq:first_derivative}}
\end{equation}
Defining $x \equiv b_i - \lambda_{i,t}$, this can be restated as follows.

\begin{alignat*}{3}
	{}					&& \tilde{w}_t + 2 \phi \theta \frac{(|x|)^\phi}{x} 	&\overset{!}{=} 0 \\
	\Leftrightarrow 	&& \frac{(|x|)^\phi}{x} 								&= - \frac{\tilde{w}_t}{2 \phi \theta} \label{eq:foc_restated} \\
\end{alignat*}
The absolute value function for any real number $x$ is defined as follows.

\begin{equation}
	|x| = \left\{
		\begin{array}{ll}
			x, \: & \: \text{if $x \geq 0$} \nonumber\\
			-x, \: & \: \text{if $x < 0$} \nonumber\\
		\end{array}
	\right.
\end{equation}
Using this definition, two cases can be distinguished when solving for the optimal task choice $\lambda^*_{i,t}$. \\

Case (1): $x \geq 0$ (i.e., $b_i \geq \lambda_{i,t}$).

\begin{alignat*}{3}
	{}				&& \frac{x^\phi}{x} 	&= - \frac{\tilde{w}_{i,t}}{2 \phi \theta} \\
	\Leftrightarrow && x					&= (- \frac{\tilde{w}_{i,t}}{2 \phi \theta})^{\frac{1}{\phi-1}}, \text{with $x = b_i - \lambda_{i,t}$} \\
	\Leftrightarrow && \lambda^*_{i,t} 		&= b_i - (- \frac{\tilde{w}_{i,t}}{2 \phi \theta})^{\frac{1}{\phi-1}}
\end{alignat*}

Case (2): $x < 0 $ (i.e., $b_i < \lambda_{i,t}$).

\begin{alignat*}{3}
	{}				&& \frac{(-x)^\phi}{x} 					&= - \frac{\tilde{w}_{i,t}}{2 \phi \theta} \\
	\Leftrightarrow && \frac{(-x)^\phi}{-x} 				&= \frac{\tilde{w}_{i,t}}{2 \phi \theta} \\
	\Leftrightarrow && - x 									&= (\frac{\tilde{w}_{i,t}}{2 \phi \theta})^\frac{1}{\phi-1}, \text{with $x = b_i - \lambda_{i,t}$} \\
	\Leftrightarrow && \lambda^*_{i,t}						&= b_i + (\frac{\tilde{w}_{i,t}}{2 \phi \theta})^\frac{1}{\phi-1} \\
\end{alignat*}
Which can be rewritten to the expression in equation (\ref{eq:lmb_opt}):
\begin{equation} \tag{\ref{eq:lmb_opt}}
	\lambda^*_{i,t} = \left\{
	\begin{array}{ll}
		b_i - (\frac{- \tilde{w}_{i,t}}{2 \phi \theta})^{\frac{1}{\phi -1}}, \: & \: \text{if $b_i \geq \lambda_{i,t}$}\\
		b_i + (\frac{\tilde{w}_{i,t}}{2 \phi \theta})^{\frac{1}{\phi - 1}}, \: & \: \text{if $b_i < \lambda_{i,t}$}
	\end{array}
\right.
\end{equation}
\end{document}